Add Result<> UTF8 back to encode/decode, refactor KMSKeyring ShouldAttemptDecryption

src/extern/dotnet/UTF8.cs
@@ -6,16 +6,28 @@ using charseq = Dafny.Sequence<char>;
 
 namespace UTF8 {
   public partial class __default {
-    public static byteseq Encode(Dafny.Sequence<char> str) {
+    public static STL.Result<byteseq> Encode(Dafny.Sequence<char> str) {
       UTF8Encoding utf8 = new UTF8Encoding(false, true);
-      byte[] utf8Bytes = utf8.GetBytes(str.Elements);
-      return byteseq.FromArray(utf8Bytes);
+      try {
+          byte[] utf8Bytes = utf8.GetBytes(str.Elements);
+          return new STL.Result_Success<byteseq>(byteseq.FromArray(utf8Bytes));
+      } catch(EncoderFallbackException e) {
+          return new STL.Result_Failure<byteseq>(charseq.FromArray("Input contains invalid Unicode characters".ToCharArray()));
+      } catch(ArgumentNullException e) {
+          return new STL.Result_Failure<byteseq>(charseq.FromArray("Input is null".ToCharArray()));
+      }
     }
 
-    public static Dafny.Sequence<char> Decode(byteseq bytes) {
+    public static STL.Result<Dafny.Sequence<char>> Decode(byteseq bytes) {
       UTF8Encoding utf8 = new UTF8Encoding(false, true);
-      string decoded = utf8.GetString(bytes.Elements);
-      return charseq.FromArray(decoded.ToCharArray());
+      try {
+          string decoded = utf8.GetString(bytes.Elements);
+          return new STL.Result_Success<Dafny.Sequence<char>>(charseq.FromArray(decoded.ToCharArray()));
+      } catch(ArgumentException e) {
+          // GetString is defined as returning ArgumentException, ArgumentNullException, DecoderFallbackException
+          // Both ArgumentNullException and DecoderFallbackException are children of ArgumentException
+          return new STL.Result_Failure<Dafny.Sequence<char>>(charseq.FromArray("Input contains an invalid Unicode code point".ToCharArray()));
+      }
     }
   }
 }
