test/Util/UTF8.dfy
@@ -6,4 +6,30 @@ module TestUTF8 {
   import opened UInt = StandardLibrary.UInt
   import opened UTF8
 
+  method {:test} EncodeHappyCase() returns (r: Result<()>) {
+    var unicodeString := "abc\u0306\u01FD\u03B2";
+    var expectedBytes := [0x61, 0x62, 0x63, 0xCC, 0x86, 0xC7, 0xBD, 0xCE, 0xB2];
+    var encoded :- UTF8.Encode(unicodeString);
+    r := RequireEqual(expectedBytes, encoded);
+  }
+
+  method {:test} EncodeInvalidUnicode() returns (r: Result<()>) {
+    // Create string with UTF-16 surrogate (\uD800)
+    var invalidUnicode := "abc\uD800";
+    var encoded := UTF8.Encode(invalidUnicode);
+    r := RequireFailure(encoded);
+  }
+
+  method {:test} DecodeHappyCase() returns (r: Result<()>) {
+    var unicodeBytes := [0x61, 0x62, 0x63, 0xCC, 0x86, 0xC7, 0xBD, 0xCE, 0xB2];
+    var expectedString := "abc\u0306\u01FD\u03B2";
+    var decoded :- UTF8.Decode(unicodeBytes);
+    r := RequireEqual(expectedString, decoded);
+  }
+
+  method {:test} DecodeInvalidUnicode() returns (r: Result<()>) {
+    // Create byte sequence with UTF-16 surrogate (0xEDA080)
+    var invalidUnicode := [0x61, 0x62, 0x63, 0xED, 0xA0, 0x80];
+    r := Require(!ValidUTF8Seq(invalidUnicode));
+  }
 }
